proofs/limit_denominator/README.md
@@ -48,7 +48,8 @@ def limit_denominator(m: int, n: int, l: int) -> tuple[int, int]:
     a, b, p, q, r, s = n, m % n, 1, 0, m // n, 1
     while 0 < b and q + a // b * s <= l:
         a, b, p, q, r, s = b, a % b, r, s, p + a // b * r, q + a // b * s
-    t, u = p + (l - q) // s * r, q + (l - q) // s * s
+    k = (l - q) // s
+    t, u = p + k * r, q + k * s
     return (r, s) if 2 * b * u <= n else (t, u)
 ```
 
@@ -364,7 +365,8 @@ def limitDenominatorSimplified (m n l : Int) : PyExcept (Int × Int) := do
   let mut (a, b, p, q, r, s) := (n, ← m % n, 1, 0, ← m // n, 1)
   while ← pure (0 < b : Bool) <&&> (do return q + (← a // b) * s ≤ l) do
     (a, b, p, q, r, s) := (b, ← a % b, r, s, p + (← a // b) * r, q + (← a // b) * s)
-  let (t, u) := (p + (← (l - q) // s) * r, q + (← (l - q) // s) * s)
+  let k ← (l - q) // s
+  let (t, u) := (p + k * r, q + k * s)
   return if 2 * b * u ≤ n then (r, s) else (t, u)
 ```
 
